WIP: Replace old Induction classes with cleaner design (not done)

Lean4Axiomatic/Integer/Impl/Difference/Induction.lean
@@ -24,15 +24,12 @@ theorem sub_eqv_diff
 
 /-- TODO -/
 def ind_diff
-    {motive : Difference ℕ → Sort u}
-    {motive_eqv : {a : Difference ℕ} → EqvOp (motive a)}
-    (on_diff : (n m : ℕ) → motive (n - m))
-    [Induction.Constraints @motive_eqv on_diff] : (a : Difference ℕ) → motive a
+    (d : Induction.Data (Difference ℕ)) : (a : Difference ℕ) → d.motive a
     := by
   intro (n——m)
-  show motive (n——m)
-  have : motive (n - m) := on_diff n m
-  have : motive (n——m) := motive_subst on_diff sub_eqv_diff this
+  show d.motive (n——m)
+  have : d.motive (n - m) := d.on_diff n m
+  have : d.motive (n——m) := d.motive_subst sub_eqv_diff this
   exact this
 
 local instance ind_ops : Induction.Ops (Difference ℕ) := {
@@ -41,60 +38,55 @@ local instance ind_ops : Induction.Ops (Difference ℕ) := {
 
 /-- TODO -/
 theorem ind_diff_subst
-    {motive : Difference ℕ → Sort u}
-    {motive_eqv : {a : Difference ℕ} → EqvOp (motive a)}
-    {on_diff : (n m : ℕ) → motive (n - m)}
-    [Induction.Constraints @motive_eqv on_diff]
-    {a₁ a₂ : Difference ℕ} (a_eqv : a₁ ≃ a₂) :
-    motive_subst on_diff ‹a₁ ≃ a₂› (ind_diff on_diff a₁) ≃ ind_diff on_diff a₂
+    (d : Induction.Data (Difference ℕ))
+    {a₁ a₂ : Difference ℕ} (a_eqv : a₁ ≃ a₂)
+    : d.motive_subst ‹a₁ ≃ a₂› (d.ind_diff a₁) ≃ d.ind_diff a₂
     := by
   revert a₁ a₂; intro (n₁——m₁) (n₂——m₂) (_ : n₁——m₁ ≃ n₂——m₂)
   let a₁ := n₁——m₁; let a₂ := n₂——m₂
-  let od₁ := on_diff n₁ m₁; let od₂ := on_diff n₂ m₂
-  let idod := ind_diff on_diff
-  show motive_subst on_diff ‹a₁ ≃ a₂› (idod a₁) ≃ idod a₂
+  let od₁ := d.on_diff n₁ m₁; let od₂ := d.on_diff n₂ m₂
+  let idod := d.ind_diff
+  show d.motive_subst ‹a₁ ≃ a₂› (d.ind_diff a₁) ≃ d.ind_diff a₂
   have diff_eqv : (n₂:Difference ℕ) - m₂ ≃ n₁ - m₁ := calc
     _ = (n₂:Difference ℕ) - m₂ := rfl
     _ ≃ n₂——m₂                 := sub_eqv_diff
     _ ≃ n₁——m₁                 := Rel.symm ‹n₁——m₁ ≃ n₂——m₂›
     _ ≃ n₁ - m₁                := Rel.symm sub_eqv_diff
   calc
-    _ = motive_subst on_diff ‹a₁ ≃ a₂› (idod a₁)
+    _ = d.motive_subst ‹a₁ ≃ a₂› (idod a₁)
       := rfl
-    _ = motive_subst on_diff ‹a₁ ≃ a₂› (motive_subst on_diff sub_eqv_diff od₁)
+    _ = d.motive_subst ‹a₁ ≃ a₂› (d.motive_subst sub_eqv_diff od₁)
       := rfl
-    _ ≃ motive_subst on_diff (Rel.trans sub_eqv_diff ‹a₁ ≃ a₂›) od₁
-      := motive_subst_compose
-    _ ≃ motive_subst on_diff (Rel.trans sub_eqv_diff ‹a₁ ≃ a₂›) (motive_subst on_diff diff_eqv od₂)
-      := Rel.symm (motive_subst_substR (on_diff_subst diff_eqv))
-    _ ≃ motive_subst on_diff (Rel.trans diff_eqv (Rel.trans sub_eqv_diff ‹a₁ ≃ a₂›)) od₂
-      := motive_subst_compose
-    _ = motive_subst on_diff sub_eqv_diff od₂
+    _ ≃ d.motive_subst (Rel.trans sub_eqv_diff ‹a₁ ≃ a₂›) od₁
+      -- TODO Hide the .C part
+      := d.C.motive_subst_compose
+    _ ≃ d.motive_subst (Rel.trans sub_eqv_diff ‹a₁ ≃ a₂›) (d.motive_subst diff_eqv od₂)
+      := Rel.symm (d.C.motive_subst_substR (d.C.on_diff_subst diff_eqv))
+    _ ≃ d.motive_subst (Rel.trans diff_eqv (Rel.trans sub_eqv_diff ‹a₁ ≃ a₂›)) od₂
+      := d.C.motive_subst_compose
+    _ = d.motive_subst sub_eqv_diff od₂
       := rfl
     _ = idod a₂
       := rfl
 
 /-- TODO -/
 theorem ind_diff_eval
-    {motive : Difference ℕ → Sort u}
-    {motive_eqv : {a : Difference ℕ} → EqvOp (motive a)}
-    {on_diff : (k j : ℕ) → motive (k - j)}
-    [Induction.Constraints @motive_eqv on_diff] {n m : ℕ} :
-    ind_diff on_diff (n - m) ≃ on_diff n m
+    (d : Induction.Data (Difference ℕ)) {n m : ℕ}
+    : d.ind_diff (n - m) ≃ d.on_diff n m
     := by
   calc
-    _ = ind_diff on_diff (n - m)
+    _ = d.ind_diff (n - m)
         := rfl
-    _ ≃ motive_subst on_diff (Rel.symm sub_eqv_diff) (ind_diff on_diff (n——m))
-        := Rel.symm (ind_diff_subst (Rel.symm sub_eqv_diff))
-    _ = motive_subst on_diff (Rel.symm sub_eqv_diff) (motive_subst on_diff sub_eqv_diff (on_diff n m))
+    _ ≃ d.motive_subst (Rel.symm sub_eqv_diff) (d.ind_diff (n——m))
+        := Rel.symm (ind_diff_subst d (Rel.symm sub_eqv_diff))
+    _ = d.motive_subst (Rel.symm sub_eqv_diff) (d.motive_subst sub_eqv_diff (d.on_diff n m))
         := rfl
-    _ ≃ motive_subst on_diff (Rel.trans sub_eqv_diff (Rel.symm sub_eqv_diff)) (on_diff n m)
-        := motive_subst_compose
-    _ = motive_subst on_diff Rel.refl (on_diff n m)
+    _ ≃ d.motive_subst (Rel.trans sub_eqv_diff (Rel.symm sub_eqv_diff)) (d.on_diff n m)
+        := d.C.motive_subst_compose
+    _ = d.motive_subst Rel.refl (d.on_diff n m)
         := rfl
-    _ ≃ on_diff n m
-        := motive_subst_refl
+    _ ≃ d.on_diff n m
+        := d.C.motive_subst_refl
 
 def ind_props : Induction.Props (Difference ℕ) := {
   ind_diff_subst := ind_diff_subst
