Lean4Axiomatic/Integer/Induction.lean
@@ -25,18 +25,17 @@ show a result holds for natural numbers than for integers.
 
 namespace Lean4Axiomatic.Integer
 
-open Relation.Equivalence (EqvOp eqvOp_prop_term)
-
-local instance eqvOp_prop_term_inst {p : Prop} : EqvOp p := eqvOp_prop_term
+open Relation.Equivalence (EqvOp)
 
 /-! ## Axioms -/
 
-/-- TODO -/
+-- TODO: merge this into Induction.lean, then see how clients need to adjust
+
+-- TODO: Operations should maybe be pulled out from properties
 class Induction.Constraints
     {ℕ : Type} [Natural ℕ]
     {ℤ : Type} [Core (ℕ := ℕ) ℤ] [Addition ℤ] [Negation ℤ] [Subtraction ℤ]
-    {motive : ℤ → Sort u} (motive_eqv : outParam ({a : ℤ} → EqvOp (motive a)))
-    (on_diff : (n m : ℕ) → motive ((n:ℤ) - (m:ℤ)))
+    (motive : ℤ → Sort u) (motive_eqv : outParam ({a : ℤ} → EqvOp (motive a)))
     :=
   /-- TODO -/
   motive_subst {a₁ a₂ : ℤ} : a₁ ≃ a₂ → motive a₁ → motive a₂
@@ -56,42 +55,105 @@ class Induction.Constraints
     motive_subst ‹a ≃ b› ma ≃ mb →
     motive_subst ‹b ≃ c› (motive_subst ‹a ≃ b› ma) ≃ motive_subst ‹b ≃ c› mb
 
+  on_diff (n m : ℕ) : motive ((n:ℤ) - (m:ℤ))
+
   /-- TODO -/
   on_diff_subst
     {n₁ m₁ n₂ m₂ : ℕ} (diff_eqv : (n₁:ℤ) - (m₁:ℤ) ≃ (n₂:ℤ) - (m₂:ℤ)) :
     motive_subst diff_eqv (on_diff n₁ m₁) ≃ on_diff n₂ m₂
 
-export Induction.Constraints (
-  on_diff_subst motive_subst motive_subst_compose motive_subst_refl
-  motive_subst_substR
-)
-
+-- TODO: What type parameters should be made explicit?
 /-- TODO -/
-class Induction.ConstConstraints
+class Induction.Data
+    {ℕ : outParam Type} [Natural ℕ]
+    (ℤ : Type) [Core (ℕ := ℕ) ℤ] [Addition ℤ] [Negation ℤ] [Subtraction ℤ]
+    :=
+  motive : ℤ → Sort u
+
+  motive_eqv {a : ℤ} : EqvOp (motive a)
+
+  C : Constraints motive motive_eqv
+
+attribute [instance] Induction.Data.motive_eqv
+
+def Induction.Data.motive_subst
     {ℕ : Type} [Natural ℕ]
     {ℤ : Type} [Core (ℕ := ℕ) ℤ] [Addition ℤ] [Negation ℤ] [Subtraction ℤ]
-    {X : Sort u} [EqvOp X] (on_diff : ℕ → ℕ → X)
-    extends Induction.Constraints (ℤ := ℤ) (λ {_} => ‹EqvOp X›) on_diff
+    (d : Data ℤ) : {a₁ a₂ : ℤ} → a₁ ≃ a₂ → motive a₁ → motive a₂
     :=
+  d.C.motive_subst
+
+def Induction.Data.on_diff
+    {ℕ : Type} [Natural ℕ]
+    {ℤ : Type} [Core (ℕ := ℕ) ℤ] [Addition ℤ] [Negation ℤ] [Subtraction ℤ]
+    (d : Data ℤ) : (n m : ℕ) → d.motive (n - m)
+    :=
+  d.C.on_diff
+
+-- TODO: What type parameters should be made explicit?
+/-- TODO -/
+class Induction.ConstData
+    {ℕ : outParam Type} [Natural ℕ]
+    (ℤ : outParam Type)
+      [Core (ℕ := ℕ) ℤ] [Addition ℤ] [Negation ℤ] [Subtraction ℤ]
+    :=
+  X : Sort u
+
+  eqv : EqvOp X
+
+  C : Constraints (ℤ := ℤ) (λ _ => X) eqv
+
   /-- TODO -/
   motive_subst_const
-    {a₁ a₂ : ℤ} (a_eqv : a₁ ≃ a₂) (x : X) : motive_subst ‹a₁ ≃ a₂› x ≃ x
+    {a₁ a₂ : ℤ} (a_eqv : a₁ ≃ a₂) (x : X) : C.motive_subst ‹a₁ ≃ a₂› x ≃ x
 
-export Induction.ConstConstraints (motive_subst_const)
+attribute [instance] Induction.ConstData.eqv
 
+def Induction.ConstData.motive_subst
+    {ℕ : Type} [Natural ℕ]
+    {ℤ : Type} [Core (ℕ := ℕ) ℤ] [Addition ℤ] [Negation ℤ] [Subtraction ℤ]
+    (cd : ConstData ℤ) : {a₁ a₂ : ℤ} → a₁ ≃ a₂ → cd.X → cd.X
+    :=
+  cd.C.motive_subst
+
+def Induction.ConstData.on_diff
+    {ℕ : Type} [Natural ℕ]
+    {ℤ : Type} [Core (ℕ := ℕ) ℤ] [Addition ℤ] [Negation ℤ] [Subtraction ℤ]
+    (cd : ConstData ℤ) : ℕ → ℕ → cd.X
+    :=
+  cd.C.on_diff
+
+/-- TODO -/
+def Induction.ConstData.toData
+    {ℕ : Type} [Natural ℕ]
+    {ℤ : Type} [Core (ℕ := ℕ) ℤ] [Addition ℤ] [Negation ℤ] [Subtraction ℤ]
+    (cd : ConstData ℤ) : Data ℤ
+    := {
+  motive := λ _ => cd.X
+  motive_eqv := cd.eqv
+  C := cd.C
+}
+
+-- TODO: Looks like with a `ℤ → Prop` motive, `on_diff` can be anything,
+-- because substitution for it is trivial. Evidence that the `on_diff` stuff
+-- should be separated out, it would make proofs much cleaner.
 def ind_constraints_prop
     {ℕ : Type} [Natural ℕ]
     {ℤ : Type} [Core (ℕ := ℕ) ℤ] [Addition ℤ] [Negation ℤ] [Subtraction ℤ]
     {motive : ℤ → Prop} {on_diff : (n m : ℕ) → motive (n - m)}
     (motive_subst : {a₁ a₂ : ℤ} → a₁ ≃ a₂ → motive a₁ → motive a₂) :
-    Induction.Constraints
-      (motive := motive) (λ {_} => eqvOp_prop_term_inst) on_diff
+    Induction.Data ℤ
     := {
-  motive_subst := motive_subst
-  motive_subst_refl := rfl
-  motive_subst_compose := rfl
-  motive_subst_substR := λ _ => rfl
-  on_diff_subst := λ _ => rfl
+  motive := motive
+  motive_eqv := Relation.Equivalence.eqvOp_prop_term
+  C := {
+    motive_subst := motive_subst
+    motive_subst_refl := rfl
+    motive_subst_compose := rfl
+    motive_subst_substR := λ _ => rfl
+    on_diff := on_diff
+    on_diff_subst := λ _ => rfl
+  }
 }
 
 def ind_constraints_const
@@ -101,14 +163,19 @@ def ind_constraints_const
     (on_diff_subst :
       {n₁ m₁ n₂ m₂ : ℕ} → (n₁:ℤ) - m₁ ≃ n₂ - m₂ →
       on_diff n₁ m₁ ≃ on_diff n₂ m₂) :
-    Induction.ConstConstraints (ℤ := ℤ) on_diff
+    Induction.ConstData ℤ
     := {
-  motive_subst := λ _ => id
+  X := X
+  eqv := ‹EqvOp X›
+  C := {
+    motive_subst := λ _ => id
+    motive_subst_refl := Rel.refl
+    motive_subst_compose := Rel.refl
+    motive_subst_substR := id
+    on_diff := on_diff
+    on_diff_subst := on_diff_subst
+  }
   motive_subst_const := λ _ _ => Rel.refl
-  motive_subst_refl := Rel.refl
-  motive_subst_compose := Rel.refl
-  motive_subst_substR := id
-  on_diff_subst := on_diff_subst
 }
 
 /-- Operations pertaining to eliminators on integers. -/
@@ -116,12 +183,21 @@ class Induction.Ops
     {ℕ : outParam Type} [Natural ℕ]
     (ℤ : Type) [Core (ℕ := ℕ) ℤ] [Addition ℤ] [Negation ℤ] [Subtraction ℤ] :=
   /-- TODO -/
-  ind_diff
-    {motive : ℤ → Sort u} {motive_eqv : {a : ℤ} → EqvOp (motive a)}
-    (on_diff : (n m : ℕ) → motive ((n:ℤ) - (m:ℤ)))
-    [Constraints @motive_eqv on_diff] (a : ℤ) : motive a
+  ind_diff (d : Data ℤ) (a : ℤ) : d.motive a
 
-export Induction.Ops (ind_diff)
+def Induction.Data.ind_diff
+    {ℕ : Type} [Natural ℕ]
+    {ℤ : Type} [Core (ℕ := ℕ) ℤ] [Addition ℤ] [Negation ℤ] [Subtraction ℤ]
+    [Ops ℤ] : (d : Data ℤ) → (a : ℤ) → d.motive a
+    :=
+  Ops.ind_diff
+
+def Induction.ConstData.ind_diff
+    {ℕ : Type} [Natural ℕ]
+    {ℤ : Type} [Core (ℕ := ℕ) ℤ] [Addition ℤ] [Negation ℤ] [Subtraction ℤ]
+    [Ops ℤ] (cd : ConstData ℤ) : ℤ → cd.X
+    :=
+  cd.toData.ind_diff
 
 /-- Properties of integer eliminators. -/
 class Induction.Props
@@ -130,19 +206,11 @@ class Induction.Props
       [Core (ℕ := ℕ) ℤ] [Addition ℤ] [Negation ℤ] [Subtraction ℤ] [ops : Ops ℤ]
     :=
   /-- TODO -/
-  ind_diff_eval
-    {motive : ℤ → Sort u} {motive_eqv : {a : ℤ} → EqvOp (motive a)}
-    {on_diff : (k j : ℕ) → motive (k - j)}
-    [Constraints @motive_eqv on_diff] {n m : ℕ} :
-    ind_diff on_diff (n - m) ≃ on_diff n m
+  ind_diff_eval (d : Data ℤ) {n m : ℕ} : d.ind_diff (n - m) ≃ d.on_diff n m
 
   ind_diff_subst
-    {motive : ℤ → Sort u} {motive_eqv : {a : ℤ} → EqvOp (motive a)}
-    {on_diff : (n m : ℕ) → motive (n - m)} [Constraints @motive_eqv on_diff]
-    {a₁ a₂ : ℤ} (a_eqv : a₁ ≃ a₂) :
-    motive_subst on_diff ‹a₁ ≃ a₂› (ind_diff on_diff a₁) ≃ ind_diff on_diff a₂
-
-export Induction.Props (ind_diff_eval ind_diff_subst)
+    (d : Data ℤ) {a₁ a₂ : ℤ} (a_eqv : a₁ ≃ a₂) :
+    d.motive_subst ‹a₁ ≃ a₂› (d.ind_diff a₁) ≃ d.ind_diff a₂
 
 /-- All integer induction/eliminator axioms. -/
 class Induction
@@ -161,88 +229,60 @@ variable {ℕ : Type} [Natural ℕ]
 variable {ℤ : Type} [Core ℤ] [Addition ℤ] [Multiplication (ℕ := ℕ) ℤ]
 variable [Negation ℤ] [Sign ℤ] [Subtraction ℤ] [Induction ℤ]
 
-/-- TODO -/
-def ind_diff_on
-    {motive : ℤ → Sort u} {motive_eqv : {a : ℤ} → EqvOp (motive a)} (a : ℤ)
-    (on_diff : (n m : ℕ) → motive ((n:ℤ) - (m:ℤ)))
-    [Induction.Constraints @motive_eqv on_diff] : motive a
+def Induction.Data.ind_diff_eval :
+    (d : Data ℤ) → {n m : ℕ} → d.ind_diff (n - m) ≃ d.on_diff n m
     :=
-  ind_diff on_diff a
+  Induction.Props.ind_diff_eval
+
+def Induction.ConstData.ind_diff_eval
+    (cd : ConstData ℤ) : {n m : ℕ} → cd.ind_diff (n - m) ≃ cd.on_diff n m
+    :=
+  cd.toData.ind_diff_eval
+
+def Induction.Data.ind_diff_subst :
+    (d : Data ℤ) → {a₁ a₂ : ℤ} → (a_eqv : a₁ ≃ a₂) →
+    d.motive_subst ‹a₁ ≃ a₂› (d.ind_diff a₁) ≃ d.ind_diff a₂
+    :=
+  Induction.Props.ind_diff_subst
+
+def Induction.ConstData.ind_diff_subst
+    (cd : ConstData ℤ) : {a₁ a₂ : ℤ} → (a_eqv : a₁ ≃ a₂) →
+    cd.motive_subst ‹a₁ ≃ a₂› (cd.ind_diff a₁) ≃ cd.ind_diff a₂
+    :=
+  cd.toData.ind_diff_subst
 
 /-- TODO -/
-theorem ind_diff_on_eval
-    {motive : ℤ → Sort u} {motive_eqv : {a : ℤ} → EqvOp (motive a)}
-    {n m : ℕ} {on_diff : (k j : ℕ) → motive ((k:ℤ) - (j:ℤ))}
-    [Induction.Constraints @motive_eqv on_diff] :
-    ind_diff_on ((n:ℤ) - (m:ℤ)) on_diff ≃ on_diff n m
+def Induction.ConstData.rec_diff
+    (cd : Induction.ConstData ℤ) : ℤ → cd.X
+    :=
+  cd.ind_diff
+
+/-- TODO -/
+theorem Induction.ConstData.rec_diff_eval
+    (cd : Induction.ConstData ℤ) {n m : ℕ} :
+    cd.rec_diff ((n:ℤ) - (m:ℤ)) ≃ cd.on_diff n m
     := calc
-  _ = ind_diff_on ((n:ℤ) - (m:ℤ)) on_diff := rfl
-  _ = ind_diff on_diff ((n:ℤ) - (m:ℤ))    := rfl
-  _ ≃ on_diff n m                         := ind_diff_eval
+  _ = cd.rec_diff ((n:ℤ) - (m:ℤ)) := rfl
+  _ = cd.ind_diff ((n:ℤ) - (m:ℤ)) := rfl
+  _ ≃ cd.on_diff n m              := cd.ind_diff_eval
 
-/-- TODO -/
-def rec_diff
-    {X : Type u} [motive_eqv : EqvOp X]
-    (on_diff : ℕ → ℕ → X)
-    [Induction.Constraints (ℤ := ℤ) (λ {_} => motive_eqv) on_diff] : ℤ → X
-    :=
-  ind_diff (motive := λ _ => X) on_diff
-
-/-- TODO -/
-theorem rec_diff_eval
-    {X : Type u} [motive_eqv : EqvOp X] {n m : ℕ} {on_diff : ℕ → ℕ → X}
-    [Induction.Constraints (ℤ := ℤ) (λ {_} => motive_eqv) on_diff] :
-    rec_diff on_diff ((n:ℤ) - (m:ℤ)) ≃ on_diff n m
-    := by
-  let diff := (n:ℤ) - (m:ℤ)
-  calc
-    _ = rec_diff on_diff diff                      := rfl
-    _ = ind_diff (motive := λ _ => X) on_diff diff := rfl
-    _ ≃ on_diff n m                                := ind_diff_eval
-
-theorem rec_diff_subst
-    {X : Type u} [EqvOp X] {on_diff : ℕ → ℕ → X} {a₁ a₂ : ℤ}
-    [Induction.ConstConstraints (ℤ := ℤ) on_diff] : a₁ ≃ a₂ →
-    rec_diff on_diff a₁ ≃ rec_diff on_diff a₂
+theorem Induction.ConstData.rec_diff_subst
+    (cd : Induction.ConstData ℤ) {a₁ a₂ : ℤ} :
+    a₁ ≃ a₂ → cd.rec_diff a₁ ≃ cd.rec_diff a₂
     := by
   intro (_ : a₁ ≃ a₂)
-  show rec_diff on_diff a₁ ≃ rec_diff on_diff a₂
+  show cd.rec_diff a₁ ≃ cd.rec_diff a₂
+  let cdid := cd.ind_diff
+  have wrap_subst : cdid a₁ ≃ cd.motive_subst ‹a₁ ≃ a₂› (cdid a₁) :=
+    Rel.symm (cd.motive_subst_const ‹a₁ ≃ a₂› (cdid a₁))
   calc
-    _ = rec_diff on_diff a₁                      := rfl
-    _ = ind_diff (motive := λ _ => X) on_diff a₁ := rfl
-    _ ≃ motive_subst (motive := λ _ => X) on_diff ‹a₁ ≃ a₂› (ind_diff (motive := λ _ => X) on_diff a₁) := Rel.symm (motive_subst_const (X := X) (on_diff := on_diff) ‹a₁ ≃ a₂› (ind_diff (motive := λ _ => X) on_diff a₁))
-    _ ≃ ind_diff (motive := λ _ => X) on_diff a₂ := ind_diff_subst (motive := λ _ => X) ‹a₁ ≃ a₂›
-    _ = rec_diff on_diff a₂                      := rfl
-
-/-- TODO -/
-def rec_diff_on
-    {X : Type u} [EqvOp X]
-    (a : ℤ) (on_diff : (n m : ℕ) → X)
-    [Induction.Constraints (ℤ := ℤ) (λ {_} => ‹EqvOp X›) on_diff] : X
-    :=
-  rec_diff on_diff a
-
-/-- TODO -/
-theorem rec_diff_on_eval
-    {X : Type u} [motive_eqv : EqvOp X] {n m : ℕ} {on_diff : ℕ → ℕ → X}
-    [Induction.Constraints (ℤ := ℤ) (λ {_} => motive_eqv) on_diff] :
-    rec_diff_on ((n:ℤ) - (m:ℤ)) on_diff ≃ on_diff n m
-    := calc
-  _ = rec_diff_on ((n:ℤ) - (m:ℤ)) on_diff := rfl
-  _ = rec_diff on_diff ((n:ℤ) - (m:ℤ))    := rfl
-  _ ≃ on_diff n m                         := rec_diff_eval
-
-theorem rec_diff_on_subst
-    {X : Type u} [motive_eqv : EqvOp X] {on_diff : ℕ → ℕ → X} {a₁ a₂ : ℤ}
-    [Induction.ConstConstraints (ℤ := ℤ) on_diff] : a₁ ≃ a₂ →
-    rec_diff_on a₁ on_diff ≃ rec_diff_on a₂ on_diff
-    := by
-  intro (_ : a₁ ≃ a₂)
-  show rec_diff_on a₁ on_diff ≃ rec_diff_on a₂ on_diff
-  calc
-    _ = rec_diff_on a₁ on_diff := rfl
-    _ = rec_diff on_diff a₁    := rfl
-    _ ≃ rec_diff on_diff a₂    := rec_diff_subst ‹a₁ ≃ a₂›
-    _ = rec_diff_on a₂ on_diff := rfl
+    -- TODO: Factor out middle steps into ind_diff_subst_const?
+    _ = cd.rec_diff a₁                      := rfl
+    _ = cd.ind_diff a₁                      := rfl
+    _ = cdid a₁                             := rfl
+    _ ≃ cd.motive_subst ‹a₁ ≃ a₂› (cdid a₁) := wrap_subst
+    _ ≃ cdid a₂                             := cd.ind_diff_subst ‹a₁ ≃ a₂›
+    _ = cd.ind_diff a₂                      := rfl
+    _ = cd.rec_diff a₂                      := rfl
 
 end Lean4Axiomatic.Integer
