Lean4Axiomatic/Integer.lean
@@ -1,6 +1,5 @@
 import Lean4Axiomatic.Integer.Exponentiation
 import Lean4Axiomatic.Integer.Induction
-import Lean4Axiomatic.Integer.InductionAlt
 import Lean4Axiomatic.Integer.Order
 
 /-!
